\documentclass[a4paper]{article}
\usepackage{amsmath}
\usepackage{amssymb}
\usepackage{enumerate}
\usepackage{physics}
\usepackage[normalem]{ulem}
\usepackage{cancel}
\begin{document}
    \begin{enumerate}[1.]
        \item $\overrightarrow{a} = 2 \times \begin{bmatrix}3 \\ 1 \end{bmatrix} - \begin{bmatrix}5 \\ 6\end{bmatrix}$\\\\
        $=  \begin{bmatrix}6 \\ 2\end{bmatrix} - \begin{bmatrix}5 \\ 6\end{bmatrix}$\\\\
        $= \begin{bmatrix}1 \\ -4\end{bmatrix}$

        \item $\overrightarrow{b} = 4 \times \begin{bmatrix}1 \\ 0 \end{bmatrix} + 3 \times \begin{bmatrix}0 \\ 1\end{bmatrix}$\\\\
        $=  \begin{bmatrix}4 \\ 0\end{bmatrix} - \begin{bmatrix}0 \\ 3\end{bmatrix}$\\\\
        $= \begin{bmatrix}4 \\ 3\end{bmatrix}$

        \item $\begin{bmatrix}-3 \\ 4\end{bmatrix}$\\\\
        $r = \sqrt{-3^2 + 4^2}$\\
        $= \sqrt{9 + 16}= 5$\\
        $\theta = \arctan (\frac{4}{-3})$\\
        $\theta=-0,93$

        \item $\begin{bmatrix}\frac{1}{\sqrt{3}} \\ \sqrt{\frac{2}{3}}\end{bmatrix}$\\\\
        $r = \sqrt{\frac{1}{\sqrt{3}}^2 + \sqrt{\frac{2}{3}}^2}= 1$\\
        $\theta = \arctan (\frac{\sqrt{\frac{2}{3}}}{\frac{1}{\sqrt{3}}})$\\
        $\theta=0,96$

        \item $\abs{\overrightarrow{a}} = \sqrt{-8^2 + -15^2}$\\
        $= \sqrt{64 + 225}$\\
        $= 17$
        $\theta = \arctan{\frac{-8}{-15}}$\\
        $= 0,49$

        \item $(1+3i)+(4+4i)\\
        =(1+4)+(3i+4i)\\
        =(5+7i)$

        \item $(2-i)+(-2+i)\\
        =(2-2)+(-i+i)\\
        =0$

        \item $(i)+(3) = 3+i$
        
        \item $(5+2i)(5-2i)\\
        = 25 -10i +10i -4\\
        =21
        $

        \item $(2-7i)(3-2i)\\
        =6-4i-21i+14i\\
        =6-25i-14i\\
        =-8-25i
        $

        \item $1+4i
        =\overline{1+4i}
        =1-4i$

        \item $\overline{-4-2i} = -4+2i$
        
        \item $1+i\\
        \abs{z} = \sqrt{1+1}\\
        = \sqrt{2}
        $

        \item $5-12i
        =\sqrt{5^2 + -12^2}\\
        =\sqrt{25+144}\\
        =\sqrt{169}\\
        =13
        $

        \item $
        5-12i\\
        r = \sqrt{2}\\
        \theta = \arctan(1)\\
        =\frac{\pi}{4}
        $

        \item $1-i\\
        r = \sqrt{2}\\
        \theta = \arctan(-1)\\
        =-\frac{\pi}{4}\\
        \sqrt{2} e^{-i\frac{\pi}{4}}\\
        $

        \item $
        r = \sqrt{25} = 5\\
        \theta = \arctan(\frac{5}{0})\\
        =\frac{\pi}{2}\\
        =3e^{i\frac{\pi}{2}}
        $

        \item $
        \overline{e^{i\frac{\pi}{2}}} = e^{-i\frac{\pi}{2}}
        $

        \item $ \overline{5e^{-i\frac{\pi}{6}}}
        =5e^{i\frac{\pi}{6}}
        $

        \item $4e^{i\pi}\\
        y = r \sin \theta\\
        = 4 \sin(\pi)\\
        = 0\\
        \\
        x = r \cos \theta \\
        = 4 \cos(\pi)\\
        = -4\\
        \\
        4(\cos(\pi) + i \sin(\pi))\\
        4(-1 + i \times 0)\\
        -4\\
        \\
        \abs{z} = \sqrt{4^2 + 0^2}\\
        = 2
        $

        \item $\beta = 7e^{i\frac{\pi}{2}}e^{-i\frac{\pi}{3}}\\
        =7(\cos(\frac{\pi}{2}) + i \sin(\frac{\pi}{2})) \times 1(\cos(\frac{\pi}{3})-i\sin(\frac{\pi}{3}))\\
        =7(1+i0) \times 1(-\frac{1}{2} - i \frac{\sqrt{3}}{2})\\
        =7 \times (-\frac{\sqrt{4}}{2}i)\\
        =7i\\
        \\
        \abs{z}=\sqrt{7^2+0^2}\\
        =\sqrt{7^2}\\
        =7
        $
    \end{enumerate}
    \subsubsection*{note: }
    \begin{enumerate}[I]
        \item $e^{i\frac{\pi}{2}} = -1$
        \item $ke^{i\theta}\\$
        for: $k = constant \hspace*{2px} \mathbb{R}, \theta = rad\\$
    \end{enumerate}
    This document write using \LaTeX \ author: Felix Montalfu(03082180055) 
\end{document}