\documentclass[a4paper]{article}
\usepackage{amsmath}
\usepackage{enumerate}
\usepackage[normalem]{ulem}
\usepackage{cancel}
\begin{document}
  \subsection*{Problem 1}
  \begin{enumerate}[i.]
    \item $\sin (\frac{\pi}{4}) $\\*
    $\frac{\pi}{4} \times \frac{180}{\pi} = 45^{\circ}$\\*
    $\sin(45^{\circ}) = \frac{\sqrt{2}}{2}$
    
    \item $\sin \frac{\pi}{2} $\\*
    $\sin(90^{\circ}) = 1$
    
    \item $\sin \frac{\pi}{3}$\\*
    $\sin(60^{\circ}) = \frac{\sqrt{3}}{2}$
    
    \item $\sin(0) = 0$
    
    \item $\cos(0) = 1$
    
    \item $\cos(\frac{\pi}{3})$\\* 
    $\cos(60^{\circ}) = \frac{1}{2}$
    
    \item $\cos(\frac{3 \pi}{4})$\\*
    $\cos(135^{\circ}) = \cos(180^{\circ} - 45^{\circ})$\\*
    $\cos(45^{\circ}) = -\frac{\sqrt{2}}{2}$
    
    \item $\cos(-\frac{\pi}{6})$\\*
    $\cos(-30^{\circ}) = \frac{\sqrt{3}}{2}$

    \item $\tan(\frac{2 \pi}{3})$\\*
    $\tan(120^{\circ}) = \tan(180^{\circ} - 60^{\circ}) = \tan(60^{\circ}) = - \sqrt{3}$

    \item $\tan(\frac{5 \pi}{4})$\\*
    $\tan(255^{\circ}) = \tan(180^{\circ} + 45^{\circ}) = \tan(45^{\circ}) = 1 $
  \end{enumerate}
  \subsection*{Problem 2}
  \begin{enumerate}[a)]
    \item 
    \begin{enumerate}[i.]
      \item $r = \sqrt{3^{2}+4^{2}} = 5$\\*
      $\tan \theta = \frac{4}{3}$\\* 
      $\theta = \arctan \frac{4}{3} = 53,13$\\*
      $(5;53,13^{\circ})$

      \item $r = \sqrt{\sqrt{3}^{2} + 1^{2}} = 2$\\*
      $\tan \theta = \frac{1}{\sqrt{3}}$\\*
      $\theta = \arctan \frac{1}{\sqrt{3}} = 30$\\*
      $(2,30^{\circ})$

      \item $r = \sqrt{(-2)^{2} + 2^{2}} = 2\sqrt{2}$\\*
      $\theta = \arctan \frac{2}{-2} = -45$\\*
      $(2\sqrt{2},-45^{\circ})$

      \item $r = \sqrt{0^{2} + 1^{2}} = 1$\\*
      $\theta = \arctan \frac{1}{0} = 90^{\circ}$\\*
      $(1,90^{\circ})$

      \item $r = \sqrt{5^{2} + 12^{2}} = 13$\\*
      $\theta = \arctan \frac{12}{5} = 67,3801^{\circ}$\\*
      $(13;67,3821^{\circ})$
    \end{enumerate}
    \item 
    \begin{enumerate}[vi.]
      \item $y = r \sin \theta$\\*
      $y = 1 \times \sin (0^{\circ}) = 0$\\*
      $x = r \cos \theta$\\*
      $x = 1 \times \cos (0^{\circ}) = 1$\\*
      $(0,1)$

      \item $\theta = 60^{\circ}$\\*
      $x = 3 \times \sin (60^{\circ}) = \frac{3\sqrt{3}}{2}$\\*
      $y = 3 \times \cos (60^{\circ}) = \frac{3}{2}$\\*
      $(\frac{3\sqrt{3}}{2};\frac{3}{2})$

      \item $\theta = 405^{\circ}$\\*
      $x = 3 \times \sin (405^{\circ}) = \frac{3\sqrt{2}}{2}$\\*
      $y = 3 \times \cos (405^{\circ}) = \frac{3\sqrt{2}}{2}$\\*
      $(\frac{3\sqrt{2}}{2};\frac{3\sqrt{2}}{2})$

      \item[ix.] $\theta = 120^{\circ}$\\*
      $x = 5 \times \sin (120^{\circ}) = \frac{5\sqrt{3}}{2}$\\*
      $y = - 5 \times \cos (120^{\circ}) = -\frac{5}{2}$\\*
      $(\frac{5\sqrt{3}}{2};-\frac{5}{2})$

      \item[x.] $\theta = 330^{\circ}$\\*
      $x = 2 \times \sin (330^{\circ}) = -\frac{2}{2} = -1$\\*
      $y = 2 \times \cos (330^{\circ}) = \frac{2\sqrt{3}}{2}$\\*
      $(-1;\frac{2\sqrt{3}}{2})$
    \end{enumerate}
  \end{enumerate}
  \subsection*{Problem 3}
  \begin{enumerate}[a)]
    \item \begin{enumerate}[i.]
      \item $\frac{x^{5} \times x^{2}}{x^{3}}$\\*\vspace*{5px}
      $= x^{4}$

      \item $e^{2} \times e^{-4}\\*$\vspace*{5px}
      $= \frac{e^{\cancel{2}^{1}}}{e^{\cancel{4}^{2}}}$\\*\vspace*{5px}
      $= \frac{1}{e^{2}}$\\*
      $= e^{-2}$
    \end{enumerate}
    \item \begin{enumerate}[i.]
      \item $x^{2}+10x$\\*
      $=x(x+10)$\vspace*{5px}

      \item $x^2 + 4x + 3$\\*
      $=(x+3)(x+1)$\vspace*{5px}

      \item $x^2 + 8x + 16$\\
      $=(x+4)(x+4)$\vspace*{5px}

      \item $x^2 - 64$\\*
      $= (x-8)(x+8)$\vspace*{5px}

      \item $x^2 - 3x - 28$\\*
      $= (x-4)(x+7)$\vspace*{5px}

      \item $\frac{e^3x^2+e^2x}{ex+1}$\\*\vspace*{5px}
      $= \frac{e^2x(\cancel{ex+1})}{\cancel{ex+1}}\\*$\vspace*{5px}
      $=e^2x$
    \end{enumerate}
  \end{enumerate}
  \subsection*{Problem 4}
  \begin{enumerate}[a)]
    \item \begin{enumerate}[i.]
      \item $\sum\limits_{k=1}^{9}k$\\*
      $= 1+2+3+4+5+6+7+8+9$\\*
      $= 45$
      \\*
      \item $\sum\limits_{k=1}^{5}k^2$\\*
      $= 1^2+2^2+3^2+4^2+5^2$\\*
      $= 55$
      \\*
      \item $\sum\limits_{k=4}^{10}(2k-1)$\\*
      $=(2 \times 4 -1)+(2 \times 5 -1)+(2 \times 6 -1)+(2 \times 7 -1)+(2 \times 8 -1)+(2 \times 9 -1)+(2 \times 10 -1)$\\*
      $= 7 + 9 + 11 +13 + 15 + 17 + 19$\\*
      $=91$
    \end{enumerate}
    \item \begin{enumerate}[i.]
      \item $\bar{x} = \frac{2 + 10 + 14 + 15 + 19 + 25}{6}$\\*
      $= 14,1667$
      \item $\bar{x} = \frac{4 + 6 + 3 + 2 + 1 0}{6}$\\*
      $= \frac{16}{6}$\\*
      $=2,6667$
    \end{enumerate}
  \end{enumerate}
  This document write using \LaTeX \ author: Felix Montalfu(03082180055)
\end{document}