\documentclass[a4paper]{article}
\usepackage{amsmath}
\usepackage{amssymb}
\usepackage{enumerate}
\usepackage{physics}
\usepackage[normalem]{ulem}
\usepackage{cancel}
\begin{document}
	\begin{enumerate}[1.]
		\item $\begin{pmatrix}5 & 2\end{pmatrix}$
		$\begin{pmatrix}6 \\ 8\end{pmatrix}$\\
		$= 30 + 16$\\
		$= 46$

		\item $\begin{pmatrix}3 & 10\end{pmatrix}$
		$\begin{pmatrix}1 \\ 7\end{pmatrix}$\\
		$= 3 + 70$\\
		$= 73$

		\item $\begin{pmatrix}1 & -2 & 4\end{pmatrix}$
		$\begin{pmatrix}2 \\ 3 \\ 3\end{pmatrix}$\\
		$=2 + -6 + 12$\\
		$=8$

		\item $\begin{pmatrix}1 & 5\end{pmatrix}$
		$\begin{pmatrix}-5 \\ 1\end{pmatrix}$\\
		$=-5 + 5$\\
		$= 0$\\\\
		$\langle \begin{pmatrix}1 \\ 5\end{pmatrix}\begin{pmatrix}-5 \\ 1\end{pmatrix}\rangle \equiv 0$

		\item $\begin{pmatrix}3 & 6 & 2\end{pmatrix}$
		$\begin{pmatrix}1 \\ 4 \\ 3\end{pmatrix}$\\\\
		$= 3+ 12+ 6$\\
		$=21$

		\item $\begin{pmatrix}5 \\ 5\end{pmatrix} = x\begin{pmatrix}1 \\ 2\end{pmatrix} + y\begin{pmatrix}3 \\1\end{pmatrix}$\\\\
		$5 = x +3y\\
		5 = 2x + y$\\\\
		\begin{tabular}{c@{\,}c@{\,}c@{\,}c@{\,}c}
			$x + 3y = 5 \abs{\cdot{2}}$\\
			$2x + y = 5 \abs{\cdot{1}}$\\
			\hline
			$2x + 6y = 10$\\
			$2x + y = 5$&-\\
			\hline
			$5y = 5$\\
			$y = 1$
		\end{tabular}
		\\\\$5 = 2x + y\\
		5 = 2x + 1\\
		5 - 1 = 2x\\
		4 = 2x\\
		x = 2$\\
		$x=2 ; y=1$

		\item $\begin{pmatrix} -7 \\ 16 \end{pmatrix}= x\begin{pmatrix}1 \\ 2\end{pmatrix} + y \begin{pmatrix}3 \\ 1\end{pmatrix}$\\
		$-7 = x + 3y\\
		16 = 2x + y$\\\\
		\begin{tabular}{c@{\,}c@{\,}c@{\,}c@{\,}c}
			$-7 = x + 3y \abs{\cdot{2}}$\\
			$16 = 2x + y \abs{\cdot{1}}$\\
			\hline
			$-14 = 2x + 6y$\\
			$16 = 2x + y$&-\\
			\hline
			$-30 = 5y$\\
			$-\frac{30}{5} = y$\\
			$-6 = y$
		\end{tabular}
		$-7 = x + -18\\
		-x = -18 + 7\\
		\cancel{-}x=\cancel{-}11\\
		x = 11\\$
		$x = 11 ; y = -6$

		\item $\begin{pmatrix}2 & 3 \\ 1 & 4\end{pmatrix}\begin{pmatrix}3 \\ -2\end{pmatrix}$\\
		$=\begin{pmatrix}(2 \cdot 3) + (3 \cdot -2) \\ (1 \cdot 3)+(4 \cdot -2)\end{pmatrix}$\\
		$=\begin{pmatrix}6 + -6 \\ 3 + -8\end{pmatrix}$\\
		$=\begin{pmatrix}0 \\ -5\end{pmatrix}$

		\item $\begin{pmatrix}1 & 4 \\ 0 & 5\end{pmatrix}\begin{pmatrix}1 \\ 1\end{pmatrix}$\\
		$=\begin{pmatrix}(1 \cdot 1)+(4 \cdot 1) \\ (1 \cdot 0) + (5 \cdot 1)\end{pmatrix}$\\
		$=\begin{pmatrix}1+4\\0+5\end{pmatrix}$\\
		$=\begin{pmatrix}5 \\ 5\end{pmatrix}$

		\item $\begin{pmatrix}-2 & 6 \\ 9 & 4\end{pmatrix}\begin{pmatrix}3 & 3 \\ -5 & 1\end{pmatrix}$\\
		$=\begin{pmatrix}(-2 \cdot 3 + 6 \cdot -5) & (-2 \cdot 3 + 6 \cdot 1) \\ (9 \cdot 3 + 4 \cdot -5) & (9 \cdot 3 + 4 \cdot 1)\end{pmatrix}$\\
		$=\begin{pmatrix}-36 & 0 \\ 7 & 31\end{pmatrix}$
	\end{enumerate}
	This document write using \LaTeX \ author: Felix Montalfu(03082180055) 
\end{document}