\documentclass[a4paper]{article}
\usepackage{amsmath}
\usepackage{amssymb}
\usepackage{enumerate}
\usepackage{physics}
\usepackage[normalem]{ulem}
\usepackage{cancel}

\begin{document}
    \begin{enumerate}[1.]
        \item $\frac{1}{4}$
        \item $\frac{1}{36}$
        \item $\frac{1}{2} \times \frac{1}{6} \\\\
        \frac{1}{12}$
        \item $\frac{1}{2} \times \frac{3}{6} \\\\
        \frac{1}{4}$
        \item $\frac{1}{2} \times (\frac{1}{6} + \frac{1}{6})\\\\
        \frac{1}{2} + \frac{2}{6}\\\\
        \frac{1}{6}$
        \item $\langle x \rangle = v \times \mathbb{P}(X = v)$\\
        $= 2 \cdot 0.1 + 5 \cdot 0.2 + 6 \cdot 0.2 + 8 \cdot 0.5$\\
        $= 0.2 + 1 + 1.2 + 4$\\
        $=6.4$
        \item $\langle x \rangle = v \times \mathbb{P}(X = v)$\\
        $=2 \cdot 0.4 + 5 \cdot 0.15 + 6 \cdot 0.35 + 8 \cdot 0.1$\\
        $= 0.8 + 0.75 + 2.1 + 0.8$\\
        $= 4.45$
        \item $Var(x) = 0.1(2)^2 + 0.2(5)^2 + 0.2(6)^2 + 0.5(8)^2 - 6.4^2$\\
        $=(0.4+5+7.2+32)-40.96$\\
        $=3.6$
        \item $Var(x) = 0.4(2)^2 + 0.15(5)^2 + 0.35(6)^2 + 0.1(8)^2 - 4.45^2$\\
        $= (1.6 + 3.75 + 12.6 + 6.4)-19.8025$\\
        $= 4.6$
        \item $P(X = 2 \hspace*{4px}and\hspace*{4px} Y = 2)$\\
        $= 0.1 \cdot 0.4$\\
        $= 0.04$
        \item $P(X = 5 \hspace*{4px}and\hspace*{4px} Y = 6)$\\
        $= 0.2 \cdot 0.35$\\
        $= 0.07$
        \item $P(X = 8 \hspace*{4px}and\hspace*{4px} Y = 5)$\\
        $= 0.5 \cdot 0.15$\\
        $= 0.075$
        \item $\ket*{\alpha} = a \begin{pmatrix}1 \\ 0\end{pmatrix}$\\
        $a \begin{pmatrix}1 & 0\end{pmatrix}$
        \item $\ket*{\beta} = a \begin{pmatrix}1 \\ 1\end{pmatrix}$\\
        $b\begin{pmatrix}1 & 1\end{pmatrix}$
        \item $\ket*{\gamma} = c \begin{pmatrix}5 \\ 3e^{i\frac{\pi}{4}}\end{pmatrix}$\\
        $c \begin{pmatrix}5 & 3e^{-i\frac{\pi}{4}}\end{pmatrix}$
        \item $\braket*{\psi}{\psi} = 1$\\
        $\braket*{\alpha}{\alpha}=1\\
        \alpha = a \begin{pmatrix}1 \\ 0\end{pmatrix}\\
        \ket*{\psi} = \frac{1}{\sqrt{\abs*{1}^2 + \abs*{0}^2}}\\
        =1$
        \item $\braket*{\beta}{\beta} = 1\\
        \ket*{\psi}=\frac{1}{\sqrt{\abs*{1}^2 + \abs*{1}^2}}\\
        =\frac{1}{\sqrt{2}}$
        \item $NP-HARD$
        \item $NP-HARD$
        \item $NP-HARD$
        \item $NP-HARD$
    \end{enumerate}
    This document write using \LaTeX \ author: Felix Montalfu(03082180055) 
\end{document}