\documentclass[a4paper]{article}
\usepackage{amsmath}
\usepackage{amssymb}
\usepackage{enumerate}
\usepackage{physics}
\usepackage[normalem]{ulem}
\usepackage{cancel}
\begin{document}
    \begin{enumerate}[1.]
        \item $\bra{A} = \begin{pmatrix}5 & 3i\end{pmatrix}$
        \item $\bra{B} = \begin{pmatrix}-7 & 4e^{i\frac{\pi}{3}}\end{pmatrix}$
        \item $\bra{C} = \begin{pmatrix} 1 \\ e^{-i\frac{\pi}{6}}\end{pmatrix}$
        \item $\braket{\psi}{\psi} = 1$
        \item $\braket{A}{A} = \\
        \ket{A} = \begin{pmatrix}5a & 3ia\end{pmatrix}\\
        \bra{A} = \begin{pmatrix}5a \\ 31a\end{pmatrix}\\
        \begin{pmatrix}5a \\ 3ia\end{pmatrix}\begin{pmatrix}5a & 3ia\end{pmatrix}\\
        25a^2 + 9 \times -1^2 \times a^2\\
        a = \frac{1}{\sqrt{34}}$
        \item $\ket{B} = \begin{pmatrix}7b \\ 4e^{-i\frac{\pi}{3}}\end{pmatrix}\\
        \bra{B} = \begin{pmatrix}7b & 4e^{i\frac{\pi}{3}}\end{pmatrix}\\
        =\begin{pmatrix}7b \\ 4e^{-i\frac{\pi}{3}}\end{pmatrix} \begin{pmatrix}7b & 4e^{-i\frac{\pi}{3}}\end{pmatrix}\\
        =49b^2 + 16 \times 1 \times b^2\\
        =\frac{1}{\sqrt{65}}$
        \item $\ket{C} = \begin{pmatrix}c & e^{i\frac{\pi}{6}}\end{pmatrix}\\
        \bra{C} = \begin{pmatrix}c \\ e^{-i\frac{\pi}{6}}\end{pmatrix}\\
        =\begin{pmatrix}c & e^{i\frac{\pi}{6}}\end{pmatrix}\begin{pmatrix}c \\ e^{-i\frac{\pi}{6}}\end{pmatrix}\\
        =c^2 + 1 \times c^2\\
        =\sqrt{1}$
        \item $\ket{0} = \begin{pmatrix}1 \\ 0\end{pmatrix}$
        \item $\ket{1} = \begin{pmatrix}0 \\ 1\end{pmatrix}$
        \item $\braket{0}{0} = \begin{pmatrix}1 \\ 0\end{pmatrix}\begin{pmatrix}1 & 0\end{pmatrix}\\
        = 1 + 0\\
        = 1$
        \item $\braket{0}{1} = \begin{pmatrix}1 \\ 0\end{pmatrix}\begin{pmatrix}0 & 1\end{pmatrix}\\
        = 0 + 0
        = 0$
        \item $\frac{1}{\sqrt{2}}(\ket{0}+\ket{1})\\
        \frac{1}{\sqrt{2}}\left(\begin{pmatrix}1 \\ 0\end{pmatrix}+\begin{pmatrix}0 \\ 1\end{pmatrix}\right)\\
        \frac{1}{\sqrt{2}}\begin{pmatrix}1 \\ 1\end{pmatrix}$
        \item $\sqrt{\frac{5}{7}}\ket{0} + \sqrt{\frac{2}{7}}\ket{1}$
        \item $P(0)=\abs{\braket{0}{+}}^2\\
        = \abs*{\frac{1}{\sqrt{2}}}^2\\\\
        = \frac{1}{2}$
        \item $P(1) = \abs{\braket{1}{-}}^2\\
        = \abs*{-\frac{1}{\sqrt{2}}}\\
        =\frac{1}{2}$
        \item $P(0) = \abs{\braket{0}{\phi}}\\
        =\abs{\frac{2}{\sqrt{13}}}^2\\
        =\frac{4}{13}$
        \item $P(1) = \abs{\braket{1}{\phi}}\\
        =\abs{\frac{3}{\sqrt{13}}e^{i\frac{\pi}{4}}}\\
        =\frac{9}{13}$
        \item $\braket{+}{+}\\
        =\left(\frac{1}{\sqrt{2}}\bra{0} + \frac{1}{\sqrt{2}}\bra{1}\right)\left(\frac{1}{\sqrt{2}}\ket{0} + \frac{1}{\sqrt{2}}\ket{1}\right)\\
        =\frac{1}{2}\cancel{\braket{0}{0}}+\frac{1}{2}\braket{0}{1}+\frac{1}{2}\braket{1}{0}+\frac{1}{2}\cancel{\braket{1}{1}}\\
        =\frac{1}{2}+\frac{1}{2}\\
        =1$
        \item $\braket{+}{-}\\
        =\left(\frac{1}{\sqrt{2}}\bra{0} + \frac{1}{\sqrt{2}}\bra{1}\right)\left(\frac{1}{\sqrt{2}}\ket{0} - \frac{1}{\sqrt{2}}\ket{1}\right)\\
        =\frac{1}{2}\cancel{\braket{0}{0}}-\frac{1}{2}\braket{0}{1}+\frac{1}{2}\braket{1}{0}-\frac{1}{2}\cancel{\braket{1}{1}}\\
        =\frac{1}{2}-\frac{1}{2}\\
        =0$
        \item $\braket{\phi}{+}\\
        =\left(\frac{2}{\sqrt{13}}\bra{0} + \frac{3}{13}e^{-i\frac{\pi}{4}}\bra{1}\right)\left(\frac{1}{\sqrt{2}}\ket{0} + \frac{1}{\sqrt{2}}\ket{1}\right)\\
        =\frac{\sqrt{2}}{13}\cancel{\braket{0}{0}}+\frac{\sqrt{2}}{13}\braket{0}{1}+\frac{3\sqrt{2}}{26}e^{-i\frac{\pi}{4}}\braket{1}{0}+\frac{3\sqrt{2}}{26}e^{-i\frac{\pi}{4}}\cancel{\braket{1}{1}}\\
        =\frac{1}{\sqrt{26}}\left(2+3e^{-i\frac{\pi}{4}}\right)\\$
        \item $\braket{-}{\phi}\\
        \left(\frac{1}{\sqrt{2}}\bra{0} - \frac{1}{\sqrt{2}}\bra{1}\right)\left(\frac{2}{\sqrt{13}}\ket{0} + \frac{3}{13}e^{-i\frac{\pi}{4}}\ket{1}\right)\\
        =-\frac{1}{\sqrt{26}}\left(2+3e^{-i\frac{\pi}{4}}\right)$
        \item $\sigma_x\ket{0}=\begin{pmatrix}0 & 1 \\ 1 & 0\end{pmatrix}\begin{pmatrix}1 \\ 0\end{pmatrix}\\
        =\begin{pmatrix}0 + 0 \\ 1 + 0\end{pmatrix}\\
        =\begin{pmatrix}0 \\ 1\end{pmatrix}\\
        =\ket{1}$
        \item $\sigma_x\ket{1}=\begin{pmatrix}0 & 1 \\1 & 0\end{pmatrix}\begin{pmatrix}0 \\ 1\end{pmatrix}\\
        =\begin{pmatrix}0+1 \\ 0+0\end{pmatrix}\\
        =\begin{pmatrix}1 \\ 0\end{pmatrix}\\
        =\ket{0}$
        \item $\sigma_y\ket{0}=\\
        =\begin{pmatrix}0-i \\ 0+0\end{pmatrix}\\
        =\begin{pmatrix}-i 0\end{pmatrix}\\
        =i\ket{0}$
        \item $\sigma_y\ket{1}=\\
        =\begin{pmatrix}0-1 \\ 0+0\end{pmatrix}\\
        =\begin{pmatrix}1 \\ 0\end{pmatrix}\\
        =i\ket{0}$
        \item $\sigma_z\ket{0}=\\
        =\begin{pmatrix}1+0 \\ 0+0\end{pmatrix}\\
        =\begin{pmatrix}1 \\ 0\end{pmatrix}\\
        =\ket{1}$
        \item $\sigma_z\ket{1}=\\
        =\begin{pmatrix}0+0 \\ 0-1\end{pmatrix}\\
        =\begin{pmatrix}0 \\ -1\end{pmatrix}\\
        =-\ket{1}$
        \item $H \ket{0}=\\
        =\frac{1}{\sqrt{2}}\begin{pmatrix}1 & 1 \\ 1 & -1\end{pmatrix}\begin{pmatrix}1 \\ 0\end{pmatrix}\\
        =\frac{1}{\sqrt{2}}\begin{pmatrix}1+0 \\ 1-0\end{pmatrix}\\
        =\frac{1}{\sqrt{2}}\begin{pmatrix}1 \\ 1\end{pmatrix}\\
        =\ket{+}$
        \item $H \ket{1}=\\
        =\frac{1}{\sqrt{2}}\begin{pmatrix}0+1 \\ 0-1\end{pmatrix}\\
        =\frac{1}{\sqrt{2}}\begin{pmatrix}1 \\ -1\end{pmatrix}\\
        =\ket{-}$
        \item $\sigma_x \ket{+}=\\
        =\sigma_x \left(\frac{1}{\sqrt{2}}\ket{0}+\frac{1}{\sqrt{2}}\ket{1}\right)\\
        =\frac{1}{\sqrt{2}}\left(\sigma_x \ket{0}+\sigma_x \ket{1}\right)\\
        =\frac{1}{\sqrt{2}}\ket{0}+\frac{1}{\sqrt{2}}\ket{1}\\
        =\ket{+}$
        \item $\sigma_x\ket{-}=\\
        =\sigma_x\left(\frac{1}{\sqrt{2}}\ket{0}+\frac{1}{\sqrt{2}}\ket{1}\right)\\
        =\frac{1}{\sqrt{2}}\left(\sigma_x\ket{0}-\sigma_x\ket{1}\right)\\
        =\frac{1}{\sqrt{2}}\left(\ket{1}+\ket{0}\right)\\
        =\ket{+}$
    \end{enumerate}
\end{document}